coq/JsInterpreter.v
@@ -2060,9 +2060,10 @@ Definition run_stat_label runs S C lab t : result :=
 Definition run_stat_with runs S C e1 t2 : result :=
   if_spec_ter (run_expr_get_value runs S C e1) (fun S1 v1 =>
     if_object (to_object S1 v1) (fun S2 l =>
-      let lex := execution_ctx_lexical_env C in
-      let '(lex', S3) := lexical_env_alloc_object S2 lex l provide_this_true in
-      let C' := execution_ctx_with_lex_this C lex' l in
+      Let lex := execution_ctx_lexical_env C in
+      Let p := lexical_env_alloc_object S2 lex l provide_this_true in
+      let '(lex', S3) := p in (* todo: let pair *)
+      Let C' := execution_ctx_with_lex_this C lex' l in
       runs_type_stat runs S3 C' t2)).
 
 Definition run_stat_if runs S C e1 t2 to : result :=
